LLVM_DS_RBT/OptionI.thy
@@ -1,0 +1,158 @@
+theory OptionI
+  imports "../../isabelle_llvm/thys/ds/LLVM_DS_All"
+  Main
+begin
+
+
+datatype 'a option_i =
+  OPTION_I (val: 'a) (flag: "1 word")
+hide_const (open) val flag
+
+instantiation option_i :: (llvm_rep) llvm_rep
+begin
+
+
+definition to_val_option_i :: "'a option_i \<Rightarrow> llvm_val" where
+  "to_val_option_i opti \<equiv> (
+    case opti of (OPTION_I x flag)  \<Rightarrow> LL_STRUCT [to_val x, to_val flag]
+  )"
+
+
+definition from_val_option_i :: "llvm_val \<Rightarrow> 'a option_i" where
+  "from_val_option_i val \<equiv> (
+    case val of
+     LL_STRUCT [x_val, flag_val] \<Rightarrow> OPTION_I (from_val x_val) (from_val flag_val)|
+      _ \<Rightarrow> undefined
+  )"
+
+
+definition "struct_of_option_i (_ :: 'a option_i itself) \<equiv> 
+  VS_STRUCT [struct_of TYPE('a), struct_of TYPE(1 word)]"
+
+
+definition "init_option_i \<equiv> OPTION_I init init" 
+
+instance
+proof(standard, goal_cases)
+  case 1
+  then show ?case
+    unfolding from_val_option_i_def to_val_option_i_def id_def
+    apply standard
+    by (auto split:  option_i.split)
+next
+  case (2 v)
+  then show ?case
+    unfolding from_val_option_i_def to_val_option_i_def struct_of_option_i_def
+    by (auto split: llvm_val.split)
+next
+  case (3 x)
+  then show ?case
+    unfolding to_val_option_i_def struct_of_option_i_def
+    by (auto split: option_i.split)
+next
+  case 4
+  then show ?case
+    unfolding to_val_option_i_def init_option_i_def struct_of_option_i_def
+    by (auto simp add: init_zero to_val_word_def)
+qed
+end
+
+
+subsubsection \<open>Setup for LLVM code export\<close>
+text \<open>Declare structure to code generator.\<close>
+lemma to_val_option_i[ll_to_val]:
+  "to_val opti = LL_STRUCT [to_val (option_i.val opti),
+                            to_val (option_i.flag opti)]"
+  by (cases opti; (simp add: to_val_option_i_def))
+  
+
+subsubsection \<open>Code Generator Preprocessor Setup\<close>  
+text \<open>The next two are auxiliary lemmas\<close>
+lemma option_i_insert_value:
+  "ll_insert_value (OPTION_I x flag) xn 0 = Mreturn (OPTION_I xn flag)"
+  "ll_insert_value (OPTION_I x flag) flagn (Suc 0) = Mreturn (OPTION_I x flagn)"
+  by (simp add:
+      ll_insert_value_def
+      llvm_insert_value_def
+      to_val_option_i_def
+      checked_from_val_def
+      struct_of_option_i_def
+      from_val_option_i_def)+
+
+
+lemma option_i_extract_value:
+  "ll_extract_value (OPTION_I x flag) 0 = Mreturn x"
+  "ll_extract_value (OPTION_I x flag) (Suc 0) = Mreturn flag"
+  by (simp add:
+      ll_extract_value_def
+      llvm_extract_value_def 
+      checked_from_val_def
+      to_val_option_i_def)+
+
+
+text \<open>Lemmas to translate node construction and destruction\<close>
+lemma inline_return_option_i[llvm_pre_simp]: "Mreturn (OPTION_I x flag) =
+   doM {
+    res \<leftarrow> ll_insert_value init x 0;
+    res \<leftarrow> ll_insert_value res flag 1;
+    Mreturn res
+  }"
+  by (auto simp: init_option_i_def option_i_insert_value)
+
+
+lemma inline_option_i_case[llvm_pre_simp]: "
+  (case opti of (OPTION_I x flag) \<Rightarrow> f x flag) =
+   doM {
+    x \<leftarrow> ll_extract_value opti 0;
+    flag \<leftarrow> ll_extract_value opti 1;
+    f x flag
+  }"  
+  apply (cases opti)
+  by (auto simp: option_i_extract_value)
+
+
+lemma inline_return_option_i_case[llvm_pre_simp]:
+ "Mreturn (case opti of (OPTION_I x flag) \<Rightarrow> f x flag) = 
+  doM {
+    x \<leftarrow> ll_extract_value opti 0;
+    flag \<leftarrow> ll_extract_value opti 1;
+    Mreturn (f x flag)   
+  }"  
+  apply (cases opti)
+  by (auto simp: option_i_extract_value)
+
+
+lemmas [llvm_inline] = option_i.val_def option_i.flag_def
+
+
+locale option_impl =
+  fixes elem_assn :: "('a, 'ai) dr_assn"
+begin
+
+
+fun option_assn' :: "'a option \<Rightarrow> 'ai option_i \<Rightarrow> ll_assn" where
+  "option_assn' None (OPTION_I xi flag) = \<up>(flag = 0)"
+| "option_assn' (Some x) (OPTION_I xi flag) = (\<up>(flag = 1) ** \<upharpoonleft>elem_assn x xi)"
+
+
+definition "option_assn \<equiv> mk_assn option_assn'"
+
+
+lemma option_assn_None [simp]: "\<upharpoonleft>option_assn None (OPTION_I xi flag) = \<up>(flag = 0)"
+  unfolding option_assn_def by auto
+
+
+lemma option_assn_Some [simp]: 
+  "\<upharpoonleft>option_assn (Some x) (OPTION_I xi flag) =(\<up>(flag = 1) ** \<upharpoonleft>elem_assn x xi)"
+  unfolding option_assn_def by auto
+
+
+lemma option_assn_0 [simp]: "\<upharpoonleft>option_assn opt (OPTION_I xi 0) = \<up>(opt = None)"
+  unfolding option_assn_def
+  by (cases opt; simp)
+
+
+end
+
+
+end
